src/proofs/ErrStateHoare.v
@@ -137,6 +137,48 @@ Proof.
   apply Hb. simpl. auto.
 Qed.
 
+Check errst_bind_dep.
+Require Import Coq.Program.Equality.
+Lemma prove_errst_spec_dep_bnd {St A B: Type} (P1 : St -> Prop) (P2: A -> St -> Prop) 
+  Q1 Q2 Q3 (a: errState St A) (b: forall (s: St) (b: A), (fst (run_errState a s) = inr b) -> errState St B):
+  (errst_spec P1 a Q1) ->
+  (forall s x Heq, errst_spec (P2 x) (b s x Heq) (Q2 x)) ->
+  (*Weaken head*)
+  (forall i, P1 i -> (forall x s2, Q1 i x s2 -> P2 x s2)) ->
+  (*Weaken rest*)
+  (forall s1 s2 s3 x y, Q1 s1 x s2 -> Q2 x s2 y s3 -> Q3 s1 y s3) ->
+  errst_spec P1 (errst_bind_dep' a b) Q3.
+Proof.
+  (*Very, very tricky due to dependent types*)
+  unfold errst_spec; simpl. intros Ha Hb Hi Himpl i z Hpi.
+  unfold errst_bind_dep'. simpl. unfold run_errState at 1. simpl.
+  unfold run_errState at 9. simpl.
+  (*Need to instantiate b with i so we can destruct [run_errState a i]*)
+  generalize dependent (Hb i).
+  generalize dependent (b i).
+  (*finally, we can destruct*)
+  destruct (run_errState a i) as [[e| x1] x2] eqn : Hrunai; simpl; [discriminate|].
+  intros bi. intros Hbi.
+
+  specialize (Ha i x1 Hpi (f_equal fst Hrunai)). intros Hz. eapply Himpl; eauto.
+  rewrite Hrunai. simpl. apply Hbi; auto.
+  eapply Hi; eauto. rewrite Hrunai in Ha. auto.
+Qed.
+
+
+(*And simpler version*)
+Lemma prove_st_spec_dep_bnd_nondep {St A B: Type} (P1 : St -> Prop)
+  Q1 Q2 Q3 a (b: forall (s: St) (b: A) , fst (run_errState a s) = inr b -> errState St B):
+  (errst_spec P1 a (fun _ => Q1)) ->
+  (forall x s Heq, errst_spec (Q1 x) (b s x Heq) (fun _ => (Q2 x))) ->
+  (*Weaken rest*)
+  (forall s2 s3 x y, Q1 x s2 -> Q2 x y s3 -> Q3 y s3) ->
+  errst_spec P1 (errst_bind_dep' a b) (fun _ => Q3).
+Proof.
+  intros Ha Hb Hw. eapply prove_errst_spec_dep_bnd
+  with (Q2:=fun x _ y s3 => Q2 x y s3); eauto.
+Qed.
+
 (*Lift state to errState*)
 Lemma errst_spec_st {A B: Type} (P: A -> Prop) 
   (Q: A -> B -> A -> Prop)
@@ -172,5 +214,45 @@ Proof.
   unfold errst_spec,errst_lift2.  simpl.
   destruct c; simpl; try discriminate.
   inversion Hc; subst. intros i b' Hp Hin. inversion Hin; subst; auto.
+Qed.
+
+(*It always suffices to just prove the implication*)
+Lemma errst_spec_err {A B: Type} (P: A -> Prop) 
+  (Q: A -> B -> A -> Prop)
+  (*state doesn't change, just need to prove Q holds*)
+  (Hpq: forall i x, P i -> Q i x i)
+  (c: errorM B):
+  errst_spec P (errst_lift2 c) Q.
+Proof.
+  destruct c.
+  - eapply errst_spec_err1; eauto.
+  - eapply errst_spec_err2; eauto.
+Qed.
+
+(*Utilities*)
+
+(*Use some assumptions in one proof, and others in another*)
+Lemma errst_spec_and {A B: Type} (P1 P2: A -> Prop) Q1 Q2 (o: errState A B):
+  errst_spec P1 o Q1 ->
+  errst_spec P2 o Q2 ->
+  errst_spec (fun i => P1 i /\ P2 i) o (fun s1 r s2 => Q1 s1 r s2 /\ Q2 s1 r s2).
+Proof.
+  unfold errst_spec. intros Hp1 Hp2 i b [Hi1 Hi2] Hrun.
+  auto.
+Qed.
+
+(*Any constant invariant is preserved*)
+Lemma errst_spec_const {A B: Type} (x: errState A B) (P1 P2: Prop):
+  (P1 -> P2) ->
+  errst_spec (fun _ => P1) x (fun _ _ _ => P2).
+Proof.
+  unfold errst_spec; auto.
+Qed.
+
+(*The precondition always holds of the initial state*)
+Lemma errst_spec_init {A B: Type} (x: errState A B) (P: A -> Prop):
+  errst_spec P x (fun s1 _ _ => P s1).
+Proof.
+  unfold errst_spec. auto.
 Qed.
 
